cleanup

Chapter 3/PBExp.thy
@@ -46,84 +46,44 @@ lemma not_preserves_value[simp]: "pbval (not_simp exp\<^sub>o) s = pbval exp\<^s
   apply(simp split: pbexp.splits)
   by auto
 
+  (* This implementation could not even be auto-proved to terminate. *)
+(* (* Converts a pbexp into NNF by pushing NOT inwards as much as possible. *)
+fun nnf :: "pbexp \<Rightarrow> pbexp" where
+  "nnf (VAR x) = (VAR x)" |
+  "nnf (NOT b) = (
+    case nnf b of
+      (NOT c)     \<Rightarrow> c |
+      (AND b1 b2) \<Rightarrow> (OR   (nnf (NOT b1)) (nnf (NOT b2))) |
+      (OR b1 b2)  \<Rightarrow> (AND  (nnf (NOT b1)) (nnf (NOT b2))) |
+      (VAR c)     \<Rightarrow> NOT (VAR c))" |  
+  "nnf (AND b1 b2) = (AND (nnf b1) (nnf b2))" |
+  "nnf (OR b1 b2) = (OR (nnf b1) (nnf b2))" *)    
+
 (* How many NOTs have been encountered so far, travelling from the expression's root to this point?
 Every time two NOTs are encountered, the count is reset to zero. *)
 datatype num_nots = ZeroN | OneN  
   
-(* Uses num_nots to simplify an expression's NOTs.   *)
-fun nnf_v2 :: "pbexp \<Rightarrow> num_nots \<Rightarrow> pbexp" where
-  "nnf_v2 (VAR x) ZeroN = (VAR x)" |
-  "nnf_v2 (VAR x) OneN = NOT (VAR x)" |
-  "nnf_v2 (NOT b) ZeroN = nnf_v2 b OneN" |
-  "nnf_v2 (NOT b) OneN = nnf_v2 b ZeroN" |
-  "nnf_v2 (AND b1 b2) ZeroN = (AND (nnf_v2 b1 ZeroN) (nnf_v2 b2 ZeroN))" |
-  "nnf_v2 (AND b1 b2) OneN = (OR (nnf_v2 b1 OneN) (nnf_v2 b2 OneN))" |
-  "nnf_v2 (OR b1 b2) ZeroN = (OR (nnf_v2 b1 ZeroN) (nnf_v2 b2 ZeroN))" |
-  "nnf_v2 (OR b1 b2) OneN = (AND (nnf_v2 b1 OneN) (nnf_v2 b2 OneN))"
+(* Convert an expression to negative normal form; pass it ZeroN   *)
+fun nnf :: "pbexp \<Rightarrow> num_nots \<Rightarrow> pbexp" where
+  "nnf (VAR x) ZeroN = (VAR x)" |
+  "nnf (VAR x) OneN = NOT (VAR x)" |
+  "nnf (NOT b) ZeroN = nnf b OneN" |
+  "nnf (NOT b) OneN = nnf b ZeroN" |
+  "nnf (AND b1 b2) ZeroN = (AND (nnf b1 ZeroN) (nnf b2 ZeroN))" |
+  "nnf (AND b1 b2) OneN = (OR (nnf b1 OneN) (nnf b2 OneN))" |
+  "nnf (OR b1 b2) ZeroN = (OR (nnf b1 ZeroN) (nnf b2 ZeroN))" |
+  "nnf (OR b1 b2) OneN = (AND (nnf b1 OneN) (nnf b2 OneN))"
 
-value "nnf_v2 (NOT (NOT (VAR ''x''))) ZeroN"
-value "nnf_v2 (NOT (NOT (NOT (VAR ''x'')))) ZeroN"
-value "nnf_v2 (NOT (NOT (NOT (NOT (VAR ''x''))))) ZeroN"
-  
-(* lemma nnf_v2_one_is_not: 
-  "pbval (nnf_v2 exp ZeroN) s = pbval exp s 
-  \<Longrightarrow> pbval (nnf_v2 exp OneN) s = (\<not> pbval exp s)"
-  apply(induction exp)
-    apply(simp_all)
- *)
+value "nnf (NOT (NOT (VAR ''x''))) ZeroN"
+value "nnf (NOT (NOT (NOT (VAR ''x'')))) ZeroN"
+value "nnf (NOT (NOT (NOT (NOT (VAR ''x''))))) ZeroN"
 
-(* lemma nnf_v2_preserves_value_1[simp]: 
-  "pbval (nnf_v2 exp num) s = 
-  (case num of ZeroN \<Rightarrow> pbval exp s | OneN \<Rightarrow> (\<not> pbval exp s))"
-  (* apply(induction exp) *)
- apply(induction exp arbitrary:num)
-    (* apply auto *)
-    apply(simp split: num_nots.splits)
- *)
-(* lemma nnf_v2_preserves_value_1: 
-  "pbval (nnf_v2 exp num) s = 
-  (case num of ZeroN \<Rightarrow> pbval exp s | OneN \<Rightarrow> (\<not> pbval exp s))"
-proof(induction exp arbitrary:num)
-  case (VAR x)
-  then show ?case 
-    by (simp split: num_nots.splits) 
-next
-  case (NOT exp)
-  then show ?case 
-    by (simp split: num_nots.splits) 
-next
-  case (AND exp1 exp2)
-  then show ?case 
-    by (simp split: num_nots.splits) 
-next
-  case (OR exp1 exp2)
-  then show ?case 
-    by (simp split: num_nots.splits) 
-qed *)
-
-(* lemma nnf_v2_preserves_value_2: 
-  "pbval (nnf_v2 exp num) s = 
-  (case num of ZeroN \<Rightarrow> pbval exp s | OneN \<Rightarrow> (\<not> pbval exp s))"
-  apply(induction exp arbitrary:num)
-     apply(simp split: num_nots.splits)
-    apply(metis PBExp.nnf_v2_preserves_value_1)
-   apply(metis PBExp.nnf_v2_preserves_value_1)
-  apply(metis PBExp.nnf_v2_preserves_value_1) *)
-    
-lemma nnf_v2_preserves_value: 
-  "pbval (nnf_v2 exp num) s = 
+lemma nnf_preserves_value: 
+  "pbval (nnf exp num) s = 
   (case num of ZeroN \<Rightarrow> pbval exp s | OneN \<Rightarrow> (\<not> pbval exp s))"
   apply(simp split: num_nots.splits)
   apply(induction exp arbitrary:num)
   by simp_all
-
-  (* Do I need to generalize ZeroN to a variable? *)
-(*  lemma nnf_v2_preserves_value[simp]: "pbval (nnf_v2 exp ZeroN) s = pbval exp s"
-  apply(induction exp)
-  (* apply(induction rule: nnf_v2.induct) *)
-    apply simp_all
-  apply(simp split: pbexp.splits) *)
-
  
 fun is_var::"pbexp \<Rightarrow> bool"  where
   "is_var (VAR _) = True"|
@@ -141,32 +101,5 @@ value "is_nnf (VAR ''x'')"
 value "is_nnf (NOT(VAR x))"  
 value "is_nnf (NOT(NOT(VAR x)))"
 
-(* (* Converts a pbexp into NNF by pushing NOT inwards as much as possible. *)
-fun nnf :: "pbexp \<Rightarrow> pbexp" where
-  "nnf (VAR x) = (VAR x)" |
-  "nnf (NOT b) = (
-    case nnf b of
-      (NOT c)     \<Rightarrow> c |
-      (AND b1 b2) \<Rightarrow> (OR   (nnf (NOT b1)) (nnf (NOT b2))) |
-      (OR b1 b2)  \<Rightarrow> (AND  (nnf (NOT b1)) (nnf (NOT b2))) |
-      (VAR c)     \<Rightarrow> NOT (VAR c))" |  
-  "nnf (AND b1 b2) = (AND (nnf b1) (nnf b2))" |
-  "nnf (OR b1 b2) = (OR (nnf b1) (nnf b2))"
-(*       (AND b1 b2) \<Rightarrow> (OR   (nnf (NOT b1)) (nnf (NOT b2))) |
-      (OR b1 b2)  \<Rightarrow> (AND  (nnf (NOT b1)) (nnf (NOT b2))) |*)  
-lemma nnf_preserves_value[simp]: "pbval (nnf exp\<^sub>o) s = pbval exp\<^sub>o s"
-  apply(induction exp\<^sub>o arbitrary: s) 
-     apply simp_all
-  nitpick
-  apply(simp split: pbexp.splits)
-  by auto
-    
-lemma nnf_is_nnf: "is_nnf (nnf b)"
-  apply(induction b)
-    nitpick
-       apply(simp_all)
-      nitpick
-  apply(simp split: pbexp.splits)
-  nitpick *)
 
 end
